$$
-\cfrac{m}{2}\cdot \cfrac{\epsilon}{2}\left(a^4\cfrac{3}{4} + 6a^2 b^2 \cos^2\phi \cdot \cfrac{1}{4} + 6a^2b^2\sin^2\phi\cdot \cfrac{1}{4}+ b^4\sin^2\phi \cdot \cfrac{3}{8} + b^4\cos^4\phi \cdot \cfrac{3}{8} + 6b^4\sin^2\phi\cos^2\phi \cdot \cfrac{1}{4}\right)
$$

$$
\cfrac{m}{4}a^2w^2 + \cfrac{9}{8}mb^2w^2 - \cfrac{m\nu^2}{4}(b^2 + a^2) - \cfrac{m\epsilon}{4}\left(a^4\cdot \cfrac{3}{8} + b^4\cdot \cfrac{3}{8} + \cfrac{3b^2a^2}{2} + b^4\cdot \cfrac{3}{16}\sin^2(2\phi)\right)
$$
$$
\cfrac{\partial S}{\partial a} = \cfrac{m}{2}aw^2 - \cfrac{m\nu^2}{2}a- \cfrac{m\epsilon}{4}\left(a^3\cdot \cfrac{3}{2}+ 3b^2a\right)
$$
$$
\cfrac{\partial S}{\partial b} = \cfrac{9}{4}mbw^2 - \cfrac{m\nu^2}{2}b - \cfrac{m\epsilon}{4}\left( b^3\cdot \cfrac{3}{2} + 3ba^2 + b^3\cdot \cfrac{3}{4}\sin^2(2\phi)\right)
$$
$$
\cfrac{\partial S}{\partial \phi} = -\cfrac{m\epsilon}{4}\left( b^4\cdot \cfrac{3}{4}\sin(2\phi)\cos(2\phi)\right)
$$


$$\begin{cases}
\cfrac{1}{2}w^2 - \cfrac{\nu^2}{2}- \cfrac{\epsilon}{4}\left(a^2\cdot \cfrac{3}{2}+ 3b^2\right) = 0 \\
\cfrac{9}{4}w^2 - \cfrac{\nu^2}{2} - \cfrac{\epsilon}{4}\left( b^2\cdot \cfrac{3}{2} + 3a^2 + b^2\cdot \cfrac{3}{4}\sin^2(2\phi)\right) = 0
\end{cases}$$

$$
22w^2 - 8\nu^2 - \epsilon\left(9a^2+ 9b^2\right) = 0
$$
$$
\cfrac{22w^2 - 8\nu^2}{9\epsilon} = a^2+ b^2
$$
$$
\cfrac{14w^2}{3\epsilon} = a^2 - b^2
$$
$$
\cfrac{4}{9}\cdot \cfrac{8w^2 - \nu^2}{\epsilon} = a^2
$$
$$
\cfrac{2\sqrt{8w^2 - \nu^2}}{3\sqrt{\epsilon}} = a
$$

1/2w^2 - v^2/2 - e/4(a^2*3/2 + 3b^2) = 0 and 9/4w^2 - v^2/2 - e/4(b^2*3/2 + 3a^2 ) = 0 for a and b 
1/2w^2 - v^2/2 - e/4(a^2*3/2 + 3b^2) = 0 and 9/4w^2 - v^2/2 - e/4(b^2*3/2 + 3a^2 + b^2 * 3/4) = 0 for a and m